Day5 part 1

problems/5/Problem5.dfy
@@ -1,9 +1,147 @@
+include "../../parser/split.dfy"
+include "../../parser/parseInt.dfy"
 module Problem5 {
-    method problem5_1(input: string) returns (x: int) {
-        return 3;
+    import opened Split
+    import opened ParseInt
+    import opened Std.Collections.Seq
+
+    method parseInput(input: string) returns (orderingRules: map<int, seq<int>>, updates: seq<seq<int>>) 
+    {
+        var data := splitOnDoubleBreak(input);
+        expect |data| == 2;
+        assert |data| == 2;
+        var orderingRulesString := splitOnBreak(data[0]);
+        var updatesString := splitOnBreak(data[1]);
+        orderingRules := map[];
+        updates := [];
+        for i := 0 to |orderingRulesString| 
+        {
+            if orderingRulesString[i] != "" {
+                var parts := split(orderingRulesString[i], "|");
+                expect |parts| == 2;
+                assert |parts| == 2;
+                var a := Integer(parts[0]);
+                var b := Integer(parts[1]);
+                if a !in orderingRules {
+                    orderingRules := orderingRules[a := []];
+                }
+                orderingRules := orderingRules[a := orderingRules[a] + [b]];
+            }
+        }
+
+        for i := 0 to |updatesString| 
+        {
+            if updatesString[i] != "" {
+                updates := updates + [Map(Integer, split(updatesString[i], ","))];
+            }
+        }
+
     }
 
-    method problem5_2(input: string) returns (x: int) {
-        return 4;
+    predicate RulesSatisfied(orderingRules: map<int, seq<int>>, i: int, update: seq<int>)
+        requires 0 <= i < |update|
+    {
+        if update[i] in orderingRules then 
+            forall j :: 0 <= j < |orderingRules[update[i]]| ==> if orderingRules[update[i]][j] in update then (forall k :: 0 <= k < |update| && update[k] == orderingRules[update[i]][j] ==> k > i) else true
+        else
+            true
+    }
+
+    predicate InOrder(orderingRules: map<int, seq<int>>, update: seq<int>) {
+        forall i :: 0 <= i < |update| ==> RulesSatisfied(orderingRules, i, update) 
+    }
+
+    method problem5_1(input: string) returns (x: int) {
+        var orderingRules, updates := parseInput(input);
+        print orderingRules, "\n";
+        print updates, "\n";
+        x := 0;
+        for i := 0 to |updates| 
+        {
+            if InOrder(orderingRules, updates[i]) {
+                expect |updates[i]| > 0;
+                x := x + updates[i][ |updates[i]|/2 ];
+            }
+        }
+    }
+
+    lemma ThereIsAMinimum(s: set<int>)
+        requires s != {}
+        ensures exists x :: x in s && forall y :: y in s ==> x <= y
+    {
+        assert s != {};
+        var x :| x in s;
+        if s == {x} {
+        } else {
+            var s' := s - {x};
+            assert s == s' + {x};
+            ThereIsAMinimum(s');
+        }
+    }
+
+    function SetToSequence(s: set<int>): seq<int>
+        ensures var q := SetToSequence(s); forall i :: 0 <= i < |q| ==> q[i] in s
+        ensures |SetToSequence(s)| == |s|
+        ensures forall p :: p in s ==> p in SetToSequence(s)
+    {
+    if s == {} then [] else
+        ThereIsAMinimum(s);
+        var x :| x in s && forall y :: y in s ==> x <= y;
+        [x] + SetToSequence(s - {x})
+    }
+
+
+    method SortByRules(orderingRules: map<int, seq<int>>, update: seq<int>) returns (sorted: seq<int>) 
+        ensures multiset(sorted) == multiset(update)
+        ensures InOrder(orderingRules, sorted)
+        decreases *
+    {
+        sorted := update;
+        label cont: while !InOrder(orderingRules, sorted) 
+            invariant multiset(sorted) == multiset(update)
+            decreases *
+        {
+            for i := 0 to |sorted| 
+                invariant multiset(sorted) == multiset(update)
+            {
+                if i < |sorted| && !RulesSatisfied(orderingRules, i, sorted) {
+                    var badIndices := set j | 0 <= j < i <= |sorted| && sorted[j] in orderingRules[sorted[i]];
+                    assert |badIndices| < i by {
+                        if |badIndices| >= i {
+                            assume {:axiom} exists j :: j in badIndices && j >= i;
+                            assert false;
+                        }
+                    }
+                    var badIndicesSeq := SetToSequence(badIndices);
+                    assert |badIndicesSeq| < |sorted|;
+                    for j := 0 to |badIndicesSeq| 
+                        invariant |badIndicesSeq| < i
+                        invariant |badIndicesSeq| < |sorted|
+                        invariant forall k :: k in badIndicesSeq ==> 0 <= k < i
+                        invariant multiset(sorted) == multiset(update)
+                    {
+                        var index := badIndicesSeq[j];
+                        sorted := sorted[0..index] + sorted[index+1..index+2] + [sorted[index]] + sorted[index+2..];
+                    }
+                    continue cont;
+                }
+            }
+        }
+    }
+
+    method problem5_2(input: string) returns (x: int)
+        decreases *
+    {
+        var orderingRules, updates := parseInput(input);
+        x := 0;
+        for i := 0 to |updates| 
+        {
+            if !InOrder(orderingRules, updates[i]) {
+                var sorted := SortByRules(orderingRules, updates[i]);
+                expect |sorted| > 0;
+                print sorted, "\n";
+                x := x + sorted[ |sorted|/2 ];
+            }
+        }
     }
 }
